Separated tag sorts (issue #5) into   * constants (`tag_const`)   * variables (`tag_var`)   * expressions (`tag_expr)`. Type `tag_const` is instanciated with `plus`, `times` and `order`. Component `tag_var` in type `instant` is possibly useless. Pending for hotfix in run derivation tactic executability (issue #2)

RunConsistency.thy
@@ -1,48 +1,46 @@
 theory RunConsistency
 imports
-    Main
     "TESL"
     "$ISABELLE_HOME/src/HOL/Eisbach/Eisbach_Tools" 
 
 begin
 
-abbreviation is_a_valuation :: "(tag \<Rightarrow> tag) \<Rightarrow> bool" where
-  "is_a_valuation \<eta> \<equiv>
-  (* A constant evaluates in itself *)
-  (\<forall>\<tau>::tag. is_concrete \<tau> \<longrightarrow> (\<eta> \<tau> = \<tau>)) \<and>
-  (* A valuation only gives concrete tags *)
-  (\<forall>\<tau>::tag. is_concrete (\<eta> \<tau>))"
-
 text \<open> A run is a time frame and tag variable valuation \<close>
   
-(* type_synonym tag_eval = "tag \<Rightarrow> tag" *)
-typedef (overloaded) tag_eval = "{ \<eta> :: tag \<Rightarrow> tag. is_a_valuation \<eta> }"
-  proof -
-    have "(\<lambda>x. case x of Unit \<Rightarrow> x | Integer _ \<Rightarrow> x | Add _ \<Rightarrow> Unit | Schematic _ \<Rightarrow> Unit) \<in> {\<eta>. is_a_valuation \<eta>}"
-      by (simp, metis tag.case(1) tag.case(2) tag.case(3) tag.case(4) tag.exhaust)
-    then show ?thesis by auto
-  qed
-type_synonym instant = "clock \<Rightarrow> (bool * tag)"
+abbreviation is_a_valuation :: "(tag_expr \<Rightarrow> tag_const) \<Rightarrow> bool" where
+  "is_a_valuation \<eta> \<equiv>
+   (* A constant valuates into itself *)
+   (\<forall>\<tau>. \<eta> \<lfloor> \<tau> \<rfloor>\<^sub>c\<^sub>s\<^sub>t = \<tau>) \<and>
+   (* Addition is distributed *)
+   (\<forall>\<tau>\<^sub>1 \<tau>\<^sub>2. \<eta> \<lfloor> \<tau>\<^sub>1 + \<tau>\<^sub>2 \<rfloor> = \<eta> \<tau>\<^sub>1 + \<eta> \<tau>\<^sub>2)"
+
+typedef (overloaded) tag_eval = "{ \<eta> :: tag_expr \<Rightarrow> tag_const. is_a_valuation \<eta> }"
+  sorry
+
+type_synonym instant = "clock \<Rightarrow> (bool * tag_var)"
 type_synonym time_frame = "nat \<Rightarrow> instant"
 type_synonym run = "time_frame * tag_eval"
 
 abbreviation hamlet where "hamlet \<equiv> fst"
 abbreviation time where "time \<equiv> snd"
 
-fun symbolic_run_interpretation_primitive :: "constr \<Rightarrow> run set" ("\<lbrakk>\<lbrakk> _ \<rbrakk>\<rbrakk>\<^sub>p\<^sub>r\<^sub>i\<^sub>m\<^sub>i\<^sub>t\<^sub>i\<^sub>v\<^sub>e") where
-    "\<lbrakk>\<lbrakk> c \<Up> n    \<rbrakk>\<rbrakk>\<^sub>p\<^sub>r\<^sub>i\<^sub>m\<^sub>i\<^sub>t\<^sub>i\<^sub>v\<^sub>e = { (\<sigma>, \<eta>). hamlet (\<sigma> n c) = True }"
-  | "\<lbrakk>\<lbrakk> c \<not>\<Up> n   \<rbrakk>\<rbrakk>\<^sub>p\<^sub>r\<^sub>i\<^sub>m\<^sub>i\<^sub>t\<^sub>i\<^sub>v\<^sub>e = { (\<sigma>, \<eta>). hamlet (\<sigma> n c) = False }"
-  | "\<lbrakk>\<lbrakk> c \<Down> n, \<tau> \<rbrakk>\<rbrakk>\<^sub>p\<^sub>r\<^sub>i\<^sub>m\<^sub>i\<^sub>t\<^sub>i\<^sub>v\<^sub>e = { (\<sigma>, \<eta>). time (\<sigma> n c) = \<tau> }"
-  | "\<lbrakk>\<lbrakk> \<doteq> (\<tau>\<^sub>1, \<alpha>, \<tau>\<^sub>2, \<beta>) \<rbrakk>\<rbrakk>\<^sub>p\<^sub>r\<^sub>i\<^sub>m\<^sub>i\<^sub>t\<^sub>i\<^sub>v\<^sub>e =
-    (* TODO: \<alpha> and \<beta> to build a semi-ring *)
-    { (\<sigma>, \<eta>). (Rep_tag_eval \<eta>) \<tau>\<^sub>1 = ((Rep_tag_eval \<eta>) \<tau>\<^sub>2)}" 
+fun symbolic_run_interpretation_primitive :: "constr \<Rightarrow> run set" ("\<lbrakk> _ \<rbrakk>\<^sub>s\<^sub>y\<^sub>m\<^sub>r\<^sub>u\<^sub>n") where
+    "\<lbrakk> c \<Up> n    \<rbrakk>\<^sub>s\<^sub>y\<^sub>m\<^sub>r\<^sub>u\<^sub>n = { (\<sigma>, \<eta>). hamlet (\<sigma> n c) = True }"
+  | "\<lbrakk> c \<not>\<Up> n   \<rbrakk>\<^sub>s\<^sub>y\<^sub>m\<^sub>r\<^sub>u\<^sub>n = { (\<sigma>, \<eta>). hamlet (\<sigma> n c) = False }"
+  | "\<lbrakk> c \<Down> n, \<tau> \<rbrakk>\<^sub>s\<^sub>y\<^sub>m\<^sub>r\<^sub>u\<^sub>n = { (\<sigma>, \<eta>).
+                      time (\<sigma> n c) = \<tau>\<^sub>v\<^sub>a\<^sub>r(c, n) \<and>
+                      ((Rep_tag_eval \<eta>) (\<lfloor>\<tau>\<^sub>v\<^sub>a\<^sub>r(c, n)\<rfloor>\<^sub>v\<^sub>a\<^sub>r)) = (case \<tau> of
+                                           \<lfloor> \<tau> \<rfloor>\<^sub>c\<^sub>s\<^sub>t \<Rightarrow> \<tau>
+                                         | \<lfloor> X \<rfloor>\<^sub>v\<^sub>a\<^sub>r \<Rightarrow> (Rep_tag_eval \<eta>) \<lfloor> X \<rfloor>\<^sub>v\<^sub>a\<^sub>r
+                                         | \<lfloor> \<tau>\<^sub>1 + \<tau>\<^sub>2 \<rfloor> \<Rightarrow> (Rep_tag_eval \<eta>) \<tau>\<^sub>1 + (Rep_tag_eval \<eta>) \<tau>\<^sub>2)}"
+  | "\<lbrakk> \<tau>\<^sub>1 \<doteq> \<alpha> * \<tau>\<^sub>2 + \<beta> \<rbrakk>\<^sub>s\<^sub>y\<^sub>m\<^sub>r\<^sub>u\<^sub>n = { (\<sigma>, \<eta>) . (Rep_tag_eval \<eta>) \<lfloor>\<tau>\<^sub>1\<rfloor>\<^sub>v\<^sub>a\<^sub>r = \<alpha> * ((Rep_tag_eval \<eta>) \<lfloor>\<tau>\<^sub>2\<rfloor>\<^sub>v\<^sub>a\<^sub>r) + \<beta>}"
 
-fun symbolic_run_interpretation :: "constr list \<Rightarrow> run set" ("\<lbrakk>\<lbrakk> _ \<rbrakk>\<rbrakk>") where
-    "\<lbrakk>\<lbrakk> [] \<rbrakk>\<rbrakk>    = { _. True }"
-  | "\<lbrakk>\<lbrakk> \<gamma> # \<Gamma> \<rbrakk>\<rbrakk> = \<lbrakk>\<lbrakk> \<gamma> \<rbrakk>\<rbrakk>\<^sub>p\<^sub>r\<^sub>i\<^sub>m\<^sub>i\<^sub>t\<^sub>i\<^sub>v\<^sub>e \<inter> \<lbrakk>\<lbrakk> \<Gamma> \<rbrakk>\<rbrakk>"
+fun symbolic_run_interpretation :: "constr list \<Rightarrow> run set" ("\<lbrakk>\<lbrakk> _ \<rbrakk>\<rbrakk>\<^sub>s\<^sub>y\<^sub>m\<^sub>r\<^sub>u\<^sub>n") where
+    "\<lbrakk>\<lbrakk> [] \<rbrakk>\<rbrakk>\<^sub>s\<^sub>y\<^sub>m\<^sub>r\<^sub>u\<^sub>n = { _. True }"
+  | "\<lbrakk>\<lbrakk> \<gamma> # \<Gamma> \<rbrakk>\<rbrakk>\<^sub>s\<^sub>y\<^sub>m\<^sub>r\<^sub>u\<^sub>n = \<lbrakk> \<gamma> \<rbrakk>\<^sub>s\<^sub>y\<^sub>m\<^sub>r\<^sub>u\<^sub>n \<inter> \<lbrakk>\<lbrakk> \<Gamma> \<rbrakk>\<rbrakk>\<^sub>s\<^sub>y\<^sub>m\<^sub>r\<^sub>u\<^sub>n"
 
 definition consistent_run :: "constr list \<Rightarrow> bool" where 
-  "consistent_run \<Gamma> \<equiv> \<exists>\<rho>. \<rho> \<in> \<lbrakk>\<lbrakk> \<Gamma> \<rbrakk>\<rbrakk>"
+  "consistent_run \<Gamma> \<equiv> \<exists>\<rho>. \<rho> \<in> \<lbrakk>\<lbrakk> \<Gamma> \<rbrakk>\<rbrakk>\<^sub>s\<^sub>y\<^sub>m\<^sub>r\<^sub>u\<^sub>n"
 
 text \<open> Defining a method for witness construction \<close>
 
@@ -58,14 +56,18 @@ abbreviation initial_run :: "run" ("\<rho>\<^sub>\<odot>") where
 fun time_frame_update :: "time_frame \<Rightarrow> constr \<Rightarrow> time_frame" ("_ \<langle> _ \<rangle>\<^sub>t\<^sub>i\<^sub>m\<^sub>e\<^sub>f\<^sub>r\<^sub>a\<^sub>m\<^sub>e") where
     "\<sigma> \<langle> c \<Up> n \<rangle>\<^sub>t\<^sub>i\<^sub>m\<^sub>e\<^sub>f\<^sub>r\<^sub>a\<^sub>m\<^sub>e = (\<lambda>n' c'. if c = c' \<and> n = n' then (True, time (\<sigma> n c)) else \<sigma> n' c')"
   | "\<sigma> \<langle> c \<not>\<Up> n \<rangle>\<^sub>t\<^sub>i\<^sub>m\<^sub>e\<^sub>f\<^sub>r\<^sub>a\<^sub>m\<^sub>e = (\<lambda>n' c'. if c = c' \<and> n = n' then (False, time (\<sigma> n c)) else \<sigma> n' c')"
-  | "\<sigma> \<langle> c \<Down> n, \<tau> \<rangle>\<^sub>t\<^sub>i\<^sub>m\<^sub>e\<^sub>f\<^sub>r\<^sub>a\<^sub>m\<^sub>e = (\<lambda>n' c'. if c = c' \<and> n = n' then (hamlet (\<sigma> n c), \<tau>) else \<sigma> n' c')"
-  | "\<sigma> \<langle> \<doteq> (\<tau>\<^sub>1, \<alpha>, \<tau>\<^sub>2, \<beta>) \<rangle>\<^sub>t\<^sub>i\<^sub>m\<^sub>e\<^sub>f\<^sub>r\<^sub>a\<^sub>m\<^sub>e = \<sigma>"
+  | "\<sigma> \<langle> c \<Down> n, \<tau> \<rangle>\<^sub>t\<^sub>i\<^sub>m\<^sub>e\<^sub>f\<^sub>r\<^sub>a\<^sub>m\<^sub>e = (\<lambda>n' c'. if c = c' \<and> n = n' then (hamlet (\<sigma> n c), \<tau>\<^sub>v\<^sub>a\<^sub>r(c, n)) else \<sigma> n' c')"
+  | "\<sigma> \<langle> \<tau>\<^sub>1 \<doteq> \<alpha> * \<tau>\<^sub>2 + \<beta> \<rangle>\<^sub>t\<^sub>i\<^sub>m\<^sub>e\<^sub>f\<^sub>r\<^sub>a\<^sub>m\<^sub>e = \<sigma>"
 
 fun tag_eval_update :: "tag_eval \<Rightarrow> constr \<Rightarrow> tag_eval" ("_ \<langle> _ \<rangle>\<^sub>t\<^sub>a\<^sub>g\<^sub>e\<^sub>v\<^sub>a\<^sub>l") where
     "\<eta> \<langle> c \<Up> n \<rangle>\<^sub>t\<^sub>a\<^sub>g\<^sub>e\<^sub>v\<^sub>a\<^sub>l = \<eta>"
   | "\<eta> \<langle> c \<not>\<Up> n \<rangle>\<^sub>t\<^sub>a\<^sub>g\<^sub>e\<^sub>v\<^sub>a\<^sub>l = \<eta>"
-  | "\<eta> \<langle> c \<Down> n, \<tau> \<rangle>\<^sub>t\<^sub>a\<^sub>g\<^sub>e\<^sub>v\<^sub>a\<^sub>l = Abs_tag_eval (\<lambda>\<tau>'. if \<tau>' = \<tau>\<^sub>v\<^sub>a\<^sub>r(c, n) then \<tau> else (Rep_tag_eval \<eta>) \<tau>')"
-  | "\<eta> \<langle> \<doteq> (\<tau>\<^sub>1, \<alpha>, \<tau>\<^sub>2, \<beta>) \<rangle>\<^sub>t\<^sub>a\<^sub>g\<^sub>e\<^sub>v\<^sub>a\<^sub>l = undefined" (* TODO *)
+  | "\<eta> \<langle> c \<Down> n, \<tau> \<rangle>\<^sub>t\<^sub>a\<^sub>g\<^sub>e\<^sub>v\<^sub>a\<^sub>l = Abs_tag_eval (\<lambda>\<tau>'. if \<tau>' = \<lfloor>\<tau>\<^sub>v\<^sub>a\<^sub>r(c, n)\<rfloor>\<^sub>v\<^sub>a\<^sub>r then (case \<tau> of
+                                             \<lfloor> \<tau> \<rfloor>\<^sub>c\<^sub>s\<^sub>t \<Rightarrow> \<tau>
+                                           | \<lfloor> X \<rfloor>\<^sub>v\<^sub>a\<^sub>r \<Rightarrow> (Rep_tag_eval \<eta>) \<lfloor> X \<rfloor>\<^sub>v\<^sub>a\<^sub>r
+                                           | \<lfloor> \<tau>\<^sub>1 + \<tau>\<^sub>2 \<rfloor> \<Rightarrow> (Rep_tag_eval \<eta>) \<tau>\<^sub>1 + (Rep_tag_eval \<eta>) \<tau>\<^sub>2
+    ) else (Rep_tag_eval \<eta>) \<tau>')"
+  | "\<eta> \<langle> \<tau>\<^sub>1 \<doteq> \<alpha> * \<tau>\<^sub>2 + \<beta> \<rangle>\<^sub>t\<^sub>a\<^sub>g\<^sub>e\<^sub>v\<^sub>a\<^sub>l = undefined" (* TODO *)
 
 fun run_update :: "run \<Rightarrow> constr \<Rightarrow> run" ("_ \<langle> _ \<rangle>") where
     "(\<sigma>, \<eta>) \<langle> \<gamma> \<rangle> = (\<sigma> \<langle> \<gamma> \<rangle>\<^sub>t\<^sub>i\<^sub>m\<^sub>e\<^sub>f\<^sub>r\<^sub>a\<^sub>m\<^sub>e, \<eta> \<langle> \<gamma> \<rangle>\<^sub>t\<^sub>a\<^sub>g\<^sub>e\<^sub>v\<^sub>a\<^sub>l)"
@@ -75,7 +77,7 @@ fun run_update' :: "constr list \<Rightarrow> run" ("\<langle>\<langle> _ \<rang
   | "\<langle>\<langle> \<gamma> # \<Gamma> \<rangle>\<rangle> = \<langle>\<langle> \<Gamma> \<rangle>\<rangle> \<langle> \<gamma> \<rangle>"
 
 lemma witness_consistency:
-  "\<langle>\<langle> \<Gamma> \<rangle>\<rangle> \<in> \<lbrakk>\<lbrakk> \<Gamma> \<rbrakk>\<rbrakk> \<Longrightarrow> consistent_run \<Gamma>"
+  "\<langle>\<langle> \<Gamma> \<rangle>\<rangle> \<in> \<lbrakk>\<lbrakk> \<Gamma> \<rbrakk>\<rbrakk>\<^sub>s\<^sub>y\<^sub>m\<^sub>r\<^sub>u\<^sub>n \<Longrightarrow> consistent_run \<Gamma>"
   unfolding consistent_run_def by (rule exI, auto)
 
 method solve_run_witness =
