TESL.thy
@@ -4,26 +4,30 @@ imports Main
 begin
 text {* We define as follows the syntax of primitives to describe symbolic runs *}
 
-(* Clocks *)
+(** Clocks **)
 datatype clock = Clk "string"        ("\<lceil> _ \<rceil>")
 type_synonym instant_index = "nat"
 
-(* Tags *) 
-datatype tag =
+(** Tags **) 
+(* Constants *)
+datatype tag_const =
     Unit                              ("\<tau>\<^sub>u\<^sub>n\<^sub>i\<^sub>t")
   | Integer   "int"                   ("\<tau>\<^sub>i\<^sub>n\<^sub>t")
-  | Schematic "clock * instant_index" ("\<tau>\<^sub>v\<^sub>a\<^sub>r")
-  | Add       "tag * tag"
-
-abbreviation is_concrete where
-  "is_concrete \<tau> \<equiv> case \<tau> of Unit \<Rightarrow> True | Integer _ \<Rightarrow> True | _ \<Rightarrow> False"
+(* Variables *)
+datatype tag_var =
+    Schematic "clock * instant_index" ("\<tau>\<^sub>v\<^sub>a\<^sub>r")
+(* Expressions *)
+datatype tag_expr =
+    Const "tag_const"           ("\<lfloor> _ \<rfloor>\<^sub>c\<^sub>s\<^sub>t")
+  | Var   "tag_var"             ("\<lfloor> _ \<rfloor>\<^sub>v\<^sub>a\<^sub>r")
+  | Add   "tag_expr" "tag_expr" ("\<lfloor> _ + _ \<rfloor>")
 
 (* Primitives for symbolic runs *)
 datatype constr =
-    Timestamp "clock" "instant_index" "tag" ("_ \<Down> _, _")
-  | Ticks     "clock" "instant_index"       ("_ \<Up> _")
-  | NotTicks  "clock" "instant_index"       ("_ \<not>\<Up> _")
-  | Affine    "tag * tag * tag * tag"       ("\<doteq>")
+    Timestamp "clock" "instant_index" "tag_expr"          ("_ \<Down> _, _")
+  | Ticks     "clock" "instant_index"                     ("_ \<Up> _")
+  | NotTicks  "clock" "instant_index"                     ("_ \<not>\<Up> _")
+  | Affine    "tag_var" "tag_const" "tag_var" "tag_const" ("_ \<doteq> _ * _ + _")
 
 type_synonym system = "constr list"
 
@@ -31,11 +35,11 @@ text{* Define as follows the syntax of TESL *}
 
 (* TESL language *)
 datatype TESL_atomic =
-    Sporadic       "clock" "tag"                 (infixr "sporadic" 55)
-  | TagRelation    "clock" "tag" "clock" "tag"   ("tag-relation _ = _ * _ + _" 55)
-  | Implies        "clock" "clock"               (infixr "implies" 55)
-  | TimeDelayedBy  "clock" "tag" "clock" "clock" ("_ time-delayed by _ on _ implies _" 55)
-  | SporadicOn     "clock" "tag" "clock"         ("_ sporadic _ on _" 55)
+    Sporadic       "clock" "tag_const"                     (infixr "sporadic" 55)
+  | TagRelation    "clock" "tag_const" "clock" "tag_const" ("tag-relation _ = _ * _ + _" 55)
+  | Implies        "clock" "clock"                         (infixr "implies" 55)
+  | TimeDelayedBy  "clock" "tag_const" "clock" "clock"     ("_ time-delayed by _ on _ implies _" 55)
+  | SporadicOn     "clock" "tag_expr" "clock"              ("_ sporadic _ on _" 55)
 
 type_synonym TESL_formula = "TESL_atomic list"
 
@@ -45,5 +49,40 @@ type_synonym TESL_formula = "TESL_atomic list"
 *)
 type_synonym TESL_ARS_conf = "system * instant_index * TESL_formula * TESL_formula"
 
+(* Instanciating tag_const to give some kind of semi-ring structure *)
+instantiation tag_const :: plus
+begin
+  fun plus_tag_const :: "tag_const \<Rightarrow> tag_const \<Rightarrow> tag_const" where
+      Unit_plus:    "Unit + Unit = Unit"
+    | Integer_plus: "(Integer n) + (Integer p) = (Integer (n + p))"
+  instance proof qed
+end
+
+instantiation tag_const :: times
+begin
+  fun times_tag_const :: "tag_const \<Rightarrow> tag_const \<Rightarrow> tag_const" where
+      Unit_times:    "Unit * Unit = Unit"
+    | Integer_times: "(Integer n) * (Integer p) = (Integer (n * p))"
+  instance proof qed
+end
+
+instantiation tag_const :: order
+begin
+  inductive less_eq_tag_const :: "tag_const \<Rightarrow> tag_const \<Rightarrow> bool" where
+    Int_less_eq[simp]:  "n \<le> m \<Longrightarrow> (Integer n) \<le> (Integer m)"
+  | Unit_less_eq[simp]: "Unit \<le> Unit"
+  definition less_tag: "(x::tag_const) < y \<longleftrightarrow> (x \<le> y) \<and> (x \<noteq> y)"
+  instance proof
+    show "\<And>x y :: tag_const. (x < y) = (x \<le> y \<and> \<not> y \<le> x)"
+      using less_eq_tag_const.simps less_tag by auto
+    show "\<And>x  :: tag_const. x \<le> x"
+      using [[smt_solver = cvc4]]
+      by (smt less_eq_tag_const.simps times_tag_const.elims)
+    show "\<And>x y z  :: tag_const. x \<le> y \<Longrightarrow> y \<le> z \<Longrightarrow> x \<le> z"
+      using less_eq_tag_const.simps by auto
+    show "\<And>x y  :: tag_const. x \<le> y \<Longrightarrow> y \<le> x \<Longrightarrow> x = y"
+      using less_eq_tag_const.simps by auto
+  qed
+end
 
 end
